More refactoring.  L3 passes regression tests.

certicoq/theories/L2_typeStripped/program.v
@@ -16,12 +16,14 @@ Local Open Scope string_scope.
 Local Open Scope bool.
 Local Open Scope list.
 Set Implicit Arguments.
-      
 
-Definition ecTrm := ecTrm Term.
+Definition ecTrm := ecTrm.
 Definition ecTyp := ecTyp Term.
 Definition ecAx := ecAx Term.
+Definition fresh := fresh.
+Hint Constructors AstCommon.fresh.
  
+(** all items in an env are application-well-formed **)
 Inductive WFaEc: envClass -> Prop :=
 | wfaecTrm: forall t, WFapp t -> WFaEc (ecTrm t)
 | wfaecTyp: forall n i, WFaEc (ecTyp n i)
@@ -33,185 +35,21 @@ Inductive WFaEnv: environ -> Prop :=
                    forall nm, WFaEnv ((nm, ec) :: p).
 Hint Constructors WFaEc WFaEnv.
 
-Inductive fresh (nm:string) : environ -> Prop :=
-| fcons: forall s p ec,
-         fresh nm p -> nm <> s -> fresh nm ((s,ec)::p)
-| fnil: fresh nm nil.
-Hint Constructors fresh.
-
-Lemma fresh_dec: forall nm p, (fresh nm p) \/ ~(fresh nm p).
-induction p.
-- left. auto.
-- destruct a. destruct IHp. destruct (string_dec nm s).
- + subst. right. intros h. inversion_Clear h. nreflexivity H4.
- + left. constructor; auto.
- + right. intros h. elim H. inversion_Clear h. assumption.
-Qed.
-
-Lemma fresh_tl: forall nm p, fresh nm p -> fresh nm (tl p).
-induction 1.
-- simpl. assumption.
-- auto.
-Qed.
-
-Lemma fresh_strengthen:
-  forall rs qs nm, fresh nm (rs++qs) -> fresh nm qs.
-induction rs; intros qs nm h.
-- assumption.
-- inversion h. subst. auto.
-Qed.
-
-Lemma fresh_not_head:
-  forall nm t p nmtp, fresh nm nmtp -> nmtp = ((nm,t)::p) -> False.
-induction 1; intros h.
-- inversion h. subst. auto.
-- discriminate h.
-Qed.
-
-
 (*** Common functions for evaluation ***)
 
 (** Lookup an entry in the environment
 *** axioms are currently not allowed
 **)
-Inductive Lookup: string -> environ -> envClass -> Prop :=
-| LHit: forall s p t, Lookup s ((s,t)::p) t
-| LMiss: forall s1 s2 p t ec,
-           s2 <> s1 -> Lookup s2 p ec -> Lookup s2 ((s1,t)::p) ec.
-Hint Constructors Lookup.
+Definition Lookup := AstCommon.Lookup.
+Hint Constructors AstCommon.Lookup.
 
-Definition LookupDfn s p t := Lookup s p (ecTrm t).
+Definition LookupDfn s p (t:Term) := Lookup s p (ecTrm t).
 Definition LookupTyp s p n i := Lookup s p (ecTyp n i).
 Definition LookupAx s p := Lookup s p ecAx.
 
 (** equivalent functions **)
-Function lookup (nm:string) (p:environ) : option envClass :=
-  match p with
-   | nil => None
-   | cons (s,ec) p => if (string_eq_bool nm s) then Some ec
-                                 else lookup nm p
-  end.
-
-Function lookupDfn (nm:string) (p:environ) : option Term :=
-  match lookup nm p with
-   | Some (AstCommon.ecTrm _ t) => Some t
-   | _ => None
-  end.
-
-Function cnstrArity (itpnm:string) (pndx:nat) (cndx:nat) (p:environ)
-                      : exception nat :=
-  match lookup itpnm p with
-    | Some (AstCommon.ecTyp _ npars itps) =>
-      arity_from_dtyp npars itps pndx cndx
-    | Some _ => raise ("L2.cnstrArity; not a type package: " ++ itpnm)
-    | none => raise ("L2.cnstrArity; datatype package not found: " ++ itpnm)
-  end.
-
-Lemma Lookup_lookup:
-  forall nm p t, Lookup nm p t -> lookup nm p = Some t.
-induction 1; intros; subst.
-- simpl. rewrite (string_eq_bool_rfl s). reflexivity.
-- simpl. rewrite (string_eq_bool_neq H). destruct t; assumption.
-Qed.
-
-Lemma lookup_Lookup:
-  forall nm p t, lookup nm p = Some t -> Lookup nm p t.
-induction p; intros t h. inversion h.
-destruct a. destruct (string_dec nm s); simpl in h.
-- subst. rewrite (string_eq_bool_rfl s) in h. 
-  injection h. intros; subst. apply LHit.
-- apply LMiss. assumption. apply IHp. 
-  rewrite (string_eq_bool_neq n) in h. assumption.
-Qed.
-
-Lemma not_lookup_not_Lookup:
- forall (nm:string) (p:environ) (ec:envClass),
-   ~(lookup nm p = Some ec) <-> ~(Lookup nm p ec).
-split; eapply deMorgan_impl.
-- apply (Lookup_lookup).
-- apply (lookup_Lookup).
-Qed.
-
-Lemma LookupDfn_lookupDfn:
-  forall nm p t, Lookup nm p t ->
-                 forall te, t = (ecTrm te) -> lookupDfn nm p = Some te.
-induction 1; intros; subst.
-- unfold lookupDfn, lookup. rewrite (string_eq_bool_rfl s). reflexivity.
-- unfold lookupDfn, lookup. rewrite (string_eq_bool_neq H). 
-  destruct t; apply IHLookup; reflexivity.
-Qed.
-
-Lemma lookupDfn_LookupDfn:
-  forall nm p t, lookupDfn nm p = Some t -> Lookup nm p (ecTrm t).
-intros nm p t. 
-functional induction (lookupDfn nm p); intros h; try discriminate.
-- injection h. intros. subst. apply lookup_Lookup. assumption.
-Qed.
-
-Lemma Lookup_single_valued:
-  forall (nm:string) (p:environ) (t r:envClass),
-    Lookup nm p t -> Lookup nm p r -> t = r.
-intros nm p t r h1 h2. 
-assert (j1:= Lookup_lookup h1 (t:=t)).
-assert (j2:= Lookup_lookup h2 (t:=r)).
-rewrite j1 in j2. injection j2; intros; subst; reflexivity. 
-Qed.
-
-Lemma LookupDfn_single_valued:
-  forall (nm:string) (p:environ) (t r:Term),
-    LookupDfn nm p t -> LookupDfn nm p r -> t = r.
-Proof.
-  unfold LookupDfn. intros nm p t r h1 h2.
-  injection (Lookup_single_valued h1 h2). intuition.
-Qed.
-
-Lemma LookupAx_lookup:
-  forall nm p, Lookup nm p ecAx -> lookup nm p = Some ecAx.
-Proof.
-  intros nm p h. inversion h; subst; simpl.
-  - rewrite (string_eq_bool_rfl nm). reflexivity.
-  - rewrite (string_eq_bool_neq H). rewrite (Lookup_lookup H0).
-    reflexivity.
-Qed.
-
-(***
-Lemma not_lookupDfn_not_LookupDfn:
- forall (nm:string) (p:environ) (t:Term),
-   ~(lookupDfn nm p = Some t) <-> ~(LookupDfn nm p t).
-split; eapply deMorgan_impl.
-- apply (proj2 (lookupDfn_LookupDfn _ _ _ )).
-- apply (proj1 (lookupDfn_LookupDfn _ _ _ )).
-Qed.
-
-Lemma lookupDfn_None_not_LookupDfn:
-  forall (nm:string) (p:environ) (t:Term),
-    lookupDfn nm p = None -> ~(LookupDfn nm p t).
-intros nm p te h. apply (proj1 (not_lookupDfn_not_LookupDfn _ _ _)). 
-intuition. rewrite h in H. discriminate.
-Qed.
-
-Lemma lookupDfn_neq:
-  forall n1 n2 p t, n1 <> n2 ->
-     lookupDfn n1 ((n2, ecConstr t) :: p) = lookupDfn n1 p.
-intros n1 n2 p t h.
-unfold lookupDfn. rewrite (string_eq_bool_neq h). reflexivity.
-Qed.
-
-Lemma LookupDfn_neq:
-  forall n1 n2 p t u, n1 <> n2 ->
-     LookupDfn n1 ((n2, ecConstr t) :: p) u -> LookupDfn n1 p u.
-intros n1 n2 p t u h1 h2.
-apply (proj1 (lookupDfn_LookupDfn _ _ _)).
-erewrite <- (lookupDfn_neq _ _ h1).
-apply (proj2 (lookupDfn_LookupDfn _ _ _)). eassumption.
-Qed.
-
-Lemma lookupDfn_eq:
-  forall n t p, lookupDfn n ((n, ecConstr t) :: p) = Some t.
-intros n t p.
-unfold lookupDfn. rewrite string_eq_bool_rfl. reflexivity.
-Qed.
-***)
+Definition lookup := @AstCommon.lookup Term.
+Definition lookupDfn := @AstCommon.lookupDfn Term.
 
 
 Lemma Lookup_pres_WFapp:
@@ -220,62 +58,6 @@ Proof.
   induction 1; intros nn ed h; inversion_Clear h.
   - assumption.
   - eapply IHWFaEnv. eassumption.
-Qed.
-
-Lemma fresh_Lookup_fails:
-  forall nm p ec, fresh nm p -> ~(Lookup nm p ec).
-induction 1; intro h; inversion h; subst; auto.
-Qed.
-
-Lemma Lookup_strengthen:
-  forall (nm1:string) pp t, Lookup nm1 pp t -> 
-       forall nm2 ec p, pp = (nm2,ec)::p -> nm1 <> nm2 -> Lookup nm1 p t.
-intros nm1 pp t h nm2 ecx px j1 j2. subst. assert (k:= Lookup_lookup h).
-simpl in k. rewrite (string_eq_bool_neq j2) in k.
-apply lookup_Lookup. assumption.
-Qed.
-
-Lemma Lookup_fresh_neq:
-  forall nm2 p t, Lookup nm2 p t -> forall nm1, fresh nm1 p -> nm1 <> nm2.
-induction 1; intros.
-- inversion H. assumption.
-- apply IHLookup. apply (fresh_tl H1).
-Qed.
-
-Lemma Lookup_weaken:
-  forall s p t, Lookup s p t -> 
-      forall nm ec, fresh nm p -> Lookup s ((nm, ec) :: p) t.
-intros s p t h1 nm ec h2.
-assert (j1:= Lookup_fresh_neq h1 h2). apply LMiss. apply neq_sym. assumption.
-assumption.
-Qed.
-
-Lemma Lookup_dec:
-  forall s p, (exists t, Lookup s p t) \/ (forall t, ~ Lookup s p t).
-Proof.
-  induction p; intros.
-  - right. intros t h. inversion h.
-  - destruct IHp; destruct a; destruct (string_dec s s0); subst.
-    + left. destruct H. exists e. apply LHit.
-    + left. destruct H. exists x. apply LMiss; assumption.
-    + destruct e.
-      * left. exists (ecTrm t). apply LHit.
-      * left. exists (ecTyp n i). apply LHit.
-      * left. exists ecAx. apply LHit.
-    + right. intros t h. inversion_Clear h. 
-      * elim n. reflexivity.
-      * elim (H t). assumption.
-Qed.
-
-Lemma fresh_lookup_None: forall nm p, fresh nm p <-> lookup nm p = None.
-split. 
-- induction 1; simpl; try reflexivity.
-  + rewrite string_eq_bool_neq; assumption.
-- induction p; auto.
-  + destruct a. destruct (string_dec nm s). 
-    * subst. simpl. rewrite string_eq_bool_rfl. discriminate.
-    * simpl. rewrite string_eq_bool_neq; try assumption. intros h.
-      apply fcons; intuition.
 Qed.
 
 
@@ -490,7 +272,8 @@ try (solve [inversion_clear j; elim (H0 nm); trivial; elim (H2 nm); trivial]);
 try (solve [inversion_clear H4; elim (H0 nm0); trivial]).
 - inversion_clear j; elim (H1 nm); trivial. elim (H3 nm); trivial.
   elim (H5 nm); trivial.
-- inversion j. subst. elim (@fresh_Lookup_fails _ _ (ecTrm pd) H2). assumption.
+- inversion j. subst. elim (@fresh_Lookup_fails _ _ _ (ecTrm pd) H2).
+  assumption.
 - inversion_Clear j. eelim (fresh_Lookup_fails H3). eassumption.
 Qed.
 
