certicoq/theories/common/AstCommon.v
@@ -6,9 +6,13 @@ Require Import Coq.PArith.BinPos.
 Require Import Coq.Strings.String.
 Require Import Coq.Arith.Peano_dec.
 Require Import Coq.Logic.Eqdep_dec.
+Require Import Coq.Lists.List.
 
 Require Import Common.RandyPrelude.
+Require Import Common.exceptionMonad.
 
+Open Scope list_scope.
+Set Implicit Arguments.
 
 Lemma name_dec: forall (s1 s2:name), {s1 = s2}+{s1 <> s2}.
 induction s1; induction s2; try (solve [right; intros h; discriminate]).
@@ -136,5 +140,211 @@ Qed.
 ***  Currently ignoring Types and Axioms **)
 Definition environ := list (string * envClass).
 Record Program : Type := mkPgm { main:trm; env:environ }.
+
+(** environments are finite functions **)
+Inductive fresh (nm:string) : environ -> Prop :=
+| fcons: forall s p ec,
+         fresh nm p -> nm <> s -> fresh nm ((s,ec)::p)
+| fnil: fresh nm nil.
+Hint Constructors fresh.
+
+Lemma fresh_dec: forall nm p, (fresh nm p) \/ ~(fresh nm p).
+induction p.
+- left. auto.
+- destruct a. destruct IHp. destruct (string_dec nm s).
+ + subst. right. intros h. inversion_Clear h. nreflexivity H4.
+ + left. constructor; auto.
+ + right. intros h. elim H. inversion_Clear h. assumption.
+Qed.
+
+Lemma fresh_tl: forall nm p, fresh nm p -> fresh nm (tl p).
+induction 1.
+- simpl. assumption.
+- auto.
+Qed.
+
+Lemma fresh_strengthen:
+  forall rs qs nm, fresh nm (rs++qs) -> fresh nm qs.
+induction rs; intros qs nm h.
+- assumption.
+- inversion h. subst. auto.
+Qed.
+
+Lemma fresh_not_head:
+  forall nm t p nmtp, fresh nm nmtp -> nmtp = ((nm,t)::p) -> False.
+induction 1; intros h.
+- inversion h. subst. auto.
+- discriminate h.
+Qed.
+
+
+(** looking a name up in an environment **)
+Inductive Lookup: string -> environ -> envClass -> Prop :=
+| LHit: forall s p t, Lookup s ((s,t)::p) t
+| LMiss: forall s1 s2 p t ec,
+           s2 <> s1 -> Lookup s2 p ec -> Lookup s2 ((s1,t)::p) ec.
+Hint Constructors Lookup.
+Definition LookupDfn s p t := Lookup s p (ecTrm t).
+Definition LookupTyp s p n i := Lookup s p (ecTyp n i).
+
+Function lookup (nm:string) (p:environ) : option envClass :=
+  match p with
+   | nil => None
+   | cons (s,ec) p => if (string_eq_bool nm s) then Some ec
+                      else lookup nm p
+  end.
+
+Definition lookupDfn (nm:string) (p:environ) : option trm :=
+  match lookup nm p with
+   | Some (ecTrm t) => Some t
+   | _ => None
+  end.
+
+Lemma Lookup_lookup:
+  forall nm p t, Lookup nm p t -> lookup nm p = Some t.
+induction 1; intros; subst.
+- simpl. rewrite (string_eq_bool_rfl s). reflexivity.
+- simpl. rewrite (string_eq_bool_neq H). destruct t; assumption.
+Qed.
+
+Lemma lookup_Lookup:
+  forall nm p t, lookup nm p = Some t -> Lookup nm p t.
+induction p; intros t h. inversion h.
+destruct a. destruct (string_dec nm s); simpl in h.
+- subst. rewrite (string_eq_bool_rfl s) in h. 
+  injection h. intros; subst. apply LHit.
+- apply LMiss. assumption. apply IHp. 
+  rewrite (string_eq_bool_neq n) in h. assumption.
+Qed.
+
+Lemma not_lookup_not_Lookup:
+ forall (nm:string) (p:environ) (ec:envClass),
+   ~(lookup nm p = Some ec) <-> ~(Lookup nm p ec).
+split; eapply deMorgan_impl.
+- apply (Lookup_lookup).
+- apply (lookup_Lookup).
+Qed.
+
+Lemma LookupDfn_lookupDfn:
+  forall nm p t, Lookup nm p t ->
+                 forall te, t = (ecTrm te) -> lookupDfn nm p = Some te.
+  induction 1; intros; subst; unfold lookupDfn, lookup.
+- rewrite (string_eq_bool_rfl s). reflexivity.
+- rewrite (string_eq_bool_neq H). 
+  destruct t; apply IHLookup; reflexivity.
+Qed.
+
+Lemma lookupDfn_LookupDfn:
+  forall nm p t, lookupDfn nm p = Some t -> Lookup nm p (ecTrm t).
+Proof.
+  intros nm p t. intros. apply lookup_Lookup.
+  unfold lookupDfn in H. 
+  case_eq (lookup nm p); intros; rewrite H0 in H.
+  - rewrite <- H0. destruct e; try discriminate. myInjection H. assumption.
+  - discriminate.
+Qed.
+
+Lemma Lookup_dec:
+  forall s p, (exists t, Lookup s p t) \/ (forall t, ~ Lookup s p t).
+Proof.
+  induction p; intros.
+  - right. intros t h. inversion h.
+  - destruct IHp; destruct a; destruct (string_dec s s0); subst.
+    + left. destruct H. exists e. apply LHit.
+    + left. destruct H. exists x. apply LMiss; assumption.
+    + destruct e.
+      * left. exists (ecTrm t). apply LHit.
+      * left. exists (ecTyp n i). apply LHit. 
+      * left. exists ecAx. apply LHit.
+    + right. intros t h. inversion_Clear h. 
+      * elim n. reflexivity.
+      * elim (H t). assumption.
+Qed.
+
+Lemma Lookup_fresh_neq:
+  forall nm2 p t, Lookup nm2 p t -> forall nm1, fresh nm1 p -> nm1 <> nm2.
+induction 1; intros.
+- inversion H. assumption.
+- apply IHLookup. apply (fresh_tl H1).
+Qed.
+
+Lemma fresh_Lookup_fails:
+  forall nm p ec, fresh nm p -> ~(Lookup nm p ec).
+induction 1; intro h; inversion h; subst; auto.
+Qed.
+
+Lemma fresh_lookup_None: forall nm p, fresh nm p <-> lookup nm p = None.
+split. 
+- induction 1; simpl; try reflexivity.
+  + rewrite string_eq_bool_neq; assumption.
+- induction p; auto.
+  + destruct a. destruct (string_dec nm s). 
+    * subst. simpl. rewrite string_eq_bool_rfl. discriminate.
+    * simpl. rewrite string_eq_bool_neq; try assumption. intros h.
+      apply fcons; intuition.
+Qed.
+
+Lemma Lookup_single_valued:
+  forall (nm:string) (p:environ) (t r:envClass),
+    Lookup nm p t -> Lookup nm p r -> t = r.
+Proof.
+  intros nm p t r h1 h2. 
+  assert (j1:= Lookup_lookup h1).
+  assert (j2:= Lookup_lookup h2).
+  rewrite j1 in j2. myInjection j2. reflexivity. 
+Qed.
+
+Lemma LookupDfn_single_valued:
+  forall (nm:string) (p:environ) (t r:trm),
+    LookupDfn nm p t -> LookupDfn nm p r -> t = r.
+Proof.
+  unfold LookupDfn. intros nm p t r h1 h2.
+  injection (Lookup_single_valued h1 h2). intuition.
+Qed.
+
+Lemma Lookup_weaken:
+  forall s p t, Lookup s p t -> 
+      forall nm ec, fresh nm p -> Lookup s ((nm, ec) :: p) t.
+intros s p t h1 nm ec h2.
+assert (j1:= Lookup_fresh_neq h1 h2). apply LMiss. apply neq_sym. assumption.
+assumption.
+Qed.
+
+Lemma Lookup_strengthen:
+  forall (nm1:string) pp t, Lookup nm1 pp t -> 
+       forall nm2 ec p, pp = (nm2,ec)::p -> nm1 <> nm2 -> Lookup nm1 p t.
+intros nm1 pp t h nm2 ecx px j1 j2. subst. assert (k:= Lookup_lookup h).
+simpl in k. rewrite (string_eq_bool_neq j2) in k.
+apply lookup_Lookup. assumption.
+Qed.
+
+
+(***
+Definition cnstrArity (itpnm:string) (pndx:nat) (cndx:nat) (p:environ)
+                      : exception nat :=
+  match lookup itpnm p with
+    | Some (ecTyp npars itps) => arity_from_dtyp npars itps pndx cndx
+    | Some _ => raise ("cnstrArity; not a type package: " ++ itpnm)
+    | none => raise ("cnstrArity; datatype package not found: " ++ itpnm)
+  end.
+ ****)
+
+(** this function for use in translation from L2 to L3 **)
+Fixpoint arity_from_dtyp
+        (npars:nat) (itps:itypPack) (tndx:nat) (cndx:nat) : exception nat :=
+  do ity <- exnNth itps tndx;
+  do itp <- exnNth (itypCnstrs ity) cndx;
+  ret (npars + (CnstrArity itp)).
+
+(** constructor arity is only computed on the fly **)
+Definition cnstrArity (p:environ) (i:inductive) (n:nat) : exception nat :=
+  match i with
+    | mkInd str m =>
+      match lookup str p with
+        | Some (ecTyp npars itps) => arity_from_dtyp npars itps m n
+        | Some _ => raise ("cnstrArity; not a type package: " ++ str)
+        | none => raise ("cnstrArity; datatype package not found: " ++ str)
+      end
+  end.
 
 End trm_Sec.
